Ski.lean
@@ -1,3 +1,4 @@
 -- This module serves as the root of the `Ski` library.
 -- Import modules here that should be built as part of the library.
+import Ski.Util
 import Ski.Basic
