Ski/Util.lean
@@ -1,0 +1,2 @@
+macro doc:(docComment)? "lemma" n:declId sig:declSig val:declVal : command =>
+  `($[$doc:docComment]? theorem $n $sig $val)
